elf/RelocElfSemantics.v
@@ -1,0 +1,219 @@
+Require Import Coqlib Integers AST Maps.
+Require Import Errors.
+Require Import Asm RelocProg RelocProgramBytes Encode.
+Require Import Memdata.
+Require Import RelocElf RelocElfgen.
+Require Import SymbolString.
+Require Import ReloctablesEncode.
+Require Import encode.Hex encode.Bits.
+Require Import SymbtableEncode SymbtableDecode.
+Require Import ReloctablesDecode.
+Import Hex Bits.
+Import ListNotations.
+
+Set Implicit Arguments.
+
+Local Open Scope error_monad_scope.
+Local Open Scope hex_scope.
+Local Open Scope bits_scope.
+Local Open Scope string_byte_scope.
+
+
+Definition get_ptr64 (ef: elf_file) : bool:=
+  match ef.(elf_head).(e_class) with
+  | ELFCLASS32 => false
+  | ELFCLASS64 => true
+  | _ => false                   (* default *)
+  end.
+
+Section WITH_FLAG.
+
+Variable elf64: bool.
+
+
+Fixpoint id_from_strtbl_aux (l: list byte) (str: list byte) :=
+  match l with
+  | b :: l' =>
+    if Byte.eq b HB["00"] then
+      match string_to_ident str with
+      | Some id =>
+        OK (id,  l')
+      | _ => Error (msg "get id from strtbl error")
+      end        
+    else id_from_strtbl_aux l' (str++[b])
+  | _ => Error (msg "get id from strtbl error")
+  end.
+  
+Definition id_from_strtbl (l: list byte) :=
+  id_from_strtbl_aux [] l.
+
+Record decode_elf_state :=
+  { dec_sectable : sectable;
+    dec_symbtable : symbtable;
+    dec_reloctable: reloctable_map;
+    dec_shstrtbl: list byte;
+    dec_strtbl: list byte
+  }.
+
+Definition update_sectable_shstrtbl st id sec shstrtbl :=
+  {| dec_sectable := PTree.set id sec st.(dec_sectable);
+     dec_symbtable := st.(dec_symbtable);
+     dec_reloctable := st.(dec_reloctable);
+     dec_shstrtbl := shstrtbl;
+     dec_strtbl := st.(dec_strtbl)
+  |}.
+
+Definition update_reloctable_shstrtbl st id reloctbl shstrtbl :=
+  {| dec_sectable := st.(dec_sectable);
+     dec_symbtable := st.(dec_symbtable);
+     dec_reloctable := PTree.set id reloctbl st.(dec_reloctable);
+     dec_shstrtbl := shstrtbl;
+     dec_strtbl := st.(dec_strtbl)
+  |}.
+
+(* skip [".strtab"] *)
+Definition update_strtbl st strtbl shstrtbl :=
+  {| dec_sectable := st.(dec_sectable);
+     dec_symbtable := st.(dec_symbtable);
+     dec_reloctable := st.(dec_reloctable);
+     dec_shstrtbl := shstrtbl;
+     dec_strtbl := strtbl
+  |}.
+
+(* skip [".symtab"] *)
+Definition update_symbtable st symbtbl shstrtbl :=
+  {| dec_sectable := st.(dec_sectable);
+     dec_symbtable := symbtbl;
+     dec_reloctable := st.(dec_reloctable);
+     dec_shstrtbl := shstrtbl;
+     dec_strtbl := st.(dec_strtbl)
+  |}.
+
+Definition acc_index_to_ident (acc: ZTree.t ident * Z) (id: ident) :=
+  let (t, idx) := acc in
+  (ZTree.set idx id t, idx + 1).
+
+Definition index_to_ident (idl: list ident) (start: Z) :=
+  fst (fold_left acc_index_to_ident idl (ZTree.empty ident, start)).
+
+
+Program Fixpoint decode_symbtable_section (l:list byte) (m:ZTree.t ident) (strtbl: list byte) (symbtbl: symbtable) {measure (length l)} : res symbtable :=
+  match l with
+  | [] => OK symbtbl
+  | _ =>
+    let len := if elf64 then 24%nat else 16%nat in
+    do (id, strtbl') <- id_from_strtbl strtbl;
+    if elf64 then
+      match take_drop len l with
+      | OK (e, r) =>      
+        do e <- decode_symbentry64 e m;
+        decode_symbtable_section r m strtbl' (PTree.set id e symbtbl)
+      | Error m => Error m
+      end     
+    else
+      match take_drop len l with
+      | OK (e, r) =>
+        do e <- decode_symbentry32 e m;
+        decode_symbtable_section r m strtbl' (PTree.set id e symbtbl)
+      | Error m => Error m
+      end
+  end.
+Next Obligation.
+  symmetry in Heq_anonymous.
+  apply take_drop_length_2 in Heq_anonymous.
+  auto.
+  destr;lia.
+Defined.
+Next Obligation.
+  symmetry in Heq_anonymous.
+  apply take_drop_length_2 in Heq_anonymous.
+  auto.
+  destr;lia.
+Defined.
+
+Program Fixpoint decode_reloctable_section (l:list byte) (m:ZTree.t ident) (reloctbl: reloctable) {measure (length l)} : res reloctable :=
+  match l with
+  | [] => OK reloctbl
+  | _ =>
+    let len := if elf64 then 16%nat else 8%nat in
+    match take_drop len l with
+    | OK (e, r) =>
+      do e <- decode_relocentry m e;
+      decode_reloctable_section r m (reloctbl ++ [e])
+    | Error m => Error m
+    end
+  end.
+Next Obligation.
+  symmetry in Heq_anonymous.
+  apply take_drop_length_2 in Heq_anonymous.
+  auto.
+  destr;lia.
+Defined.
+
+  
+Definition acc_section_header (st: res decode_elf_state) (sec_h: section * section_header) :=
+  do st <- st;
+  let (sec, h) := sec_h in
+  match h.(sh_type) with
+
+  (* code and data *)
+  | SHT_PROGBITS =>
+    (* get section id *)
+    do (id, shstrtbl') <- id_from_strtbl st.(dec_shstrtbl);
+    match h.(sh_flags) with
+    | [SHF_ALLOC] =>
+      OK (update_sectable_shstrtbl st id (sec_rodata sec) shstrtbl')
+    | [SHF_ALLOC; SHF_WRITE] =>
+      OK (update_sectable_shstrtbl st id (sec_rwdata sec) shstrtbl')
+    | [SHF_ALLOC; SHF_EXECINSTR] =>
+      OK (update_sectable_shstrtbl st id (sec_text sec) shstrtbl')
+    | _ => Error (msg "sh_flag error")
+    end
+       
+  (* restore the strtbl in state*)
+  (* shstrtbl impossible, since we removelast the shstrtbl header *)
+  | SHT_STRTAB =>
+    do (_, shstrtbl') <- take_drop (length strtab_str) st.(dec_shstrtbl);
+    OK (update_strtbl st sec shstrtbl')
+                  
+  (* symbtable *)
+  | SHT_SYMTAB =>
+    (* get id to index map from sectable: Z -> ident *)
+    let idl_sectbl := PTree.elements st.(dec_sectable) in
+    let secidl := map fst idl_sectbl in
+    let secidxmap := index_to_ident secidl 1 in
+    (* iterate symbtable section and strtable simutaneously *)
+    do symbtbl <- decode_symbtable_section sec secidxmap st.(dec_strtbl) (PTree.empty symbentry);
+    do (_, shstrtbl') <- take_drop (length symtab_str) st.(dec_shstrtbl);
+    OK (update_symbtable st symbtbl shstrtbl')
+       
+  | SHT_REL =>
+    (* get id to index map from sectable: Z -> ident *)
+    let idl_sectbl := PTree.elements st.(dec_sectable) in
+    let secidl := map fst idl_sectbl in
+    let secidxmap := index_to_ident secidl 1 in
+    do (_, shstrtbl0) <- take_drop (length SB[".rel"]) st.(dec_shstrtbl);
+    do (id, shstrtbl') <- id_from_strtbl shstrtbl0;
+    do reloctbl <- decode_reloctable_section sec secidxmap [];
+    OK (update_reloctable_shstrtbl st id reloctbl shstrtbl')
+           
+  | _ => Error (msg "unsupported section header")
+  end.
+
+End WITH_FLAG.
+
+Definition init_dec_state shstrtbl :=
+  {| dec_sectable := PTree.empty RelocProgramBytes.section;
+     dec_symbtable := PTree.empty symbentry;
+     dec_reloctable := PTree.empty reloctable;
+     dec_shstrtbl := shstrtbl;
+     dec_strtbl := [] |}.
+
+Definition decode_elf (p: elf_file) : res program :=
+  let init := init_dec_state (last p.(elf_sections) []) in
+  let elf64 := get_ptr64 p in
+  let secs := removelast p.(elf_sections) in
+  let hs := tail (removelast p.(elf_section_headers)) in
+  do st <- fold_left (acc_section_header elf64) (combine secs hs) (OK init);
+  OK (Build_program _ _ _ _ p.(prog_defs) p.(prog_public) p.(prog_main) st.(dec_sectable) st.(dec_symbtable) st.(dec_reloctable) p.(prog_senv)).
+
