elf/ReloctablesDecode.v
@@ -1,0 +1,118 @@
+Require Import Coqlib Integers AST Maps.
+Require Import Asm.
+Require Import Errors.
+Require Import RelocProg RelocProgramBytes Encode.
+Require Import Memdata.
+Require Import encode.Hex encode.Bits.
+Import Hex Bits.
+Import ListNotations.
+Require Import SymbtableDecode ReloctablesEncode.
+Set Implicit Arguments.
+
+Local Open Scope error_monad_scope.
+Local Open Scope hex_scope.
+Local Open Scope bits_scope.
+Local Open Scope Z_scope.
+
+Definition decode_reloctype (z: Z) : res reloctype :=
+  match z with
+  | 0 => OK reloc_null
+  | 1 => OK reloc_abs
+  | 2 => OK reloc_rel
+  | _ => Error (msg "decode_reloctype: Unexpected value for symbtype")
+  end.
+
+Lemma decode_encode_reloctype rt:
+  decode_reloctype (encode_reloctype rt) = OK rt.
+Proof. destruct rt; reflexivity. Qed.
+
+Definition decode_reloc_info (m: ZTree.t ident) (lb: list byte) : res (reloctype * ident) :=
+  if Archi.ptr64 then
+    let z := decode_int lb in
+    do rt <- decode_reloctype (z mod Z.pow 2 32);
+    let symb := z / (Z.pow 2 32) in
+    match ZTree.get symb m with
+    | Some id =>
+      OK (rt, id)
+    | _ => Error (msg "no ident in decode_reloc_info")
+    end
+  else
+    let z := decode_int lb in
+    do rt <- decode_reloctype (z mod Z.pow 2 8);
+    let symb := z / (Z.pow 2 8) in
+    match ZTree.get symb m with
+    | Some id =>
+      OK (rt, id)
+    | _ => Error (msg "no ident in decode_reloc_info")
+    end.
+
+
+
+Lemma decode_encode_reloc_info: forall bs rt symb m1 m2 (M: match_idxmap m1 m2),
+    encode_reloc_info m1 rt symb = OK bs ->
+    decode_reloc_info m2 bs = OK (rt, symb).
+Proof.
+  unfold decode_reloc_info, encode_reloc_info, match_idxmap.
+  intros.
+  destr_in H. apply M in Heqo.
+  destr.
+  - destr_in H.
+    inv H. unfold encode_int64.
+    rewrite decode_encode_int.
+    simpl.
+    rewrite Z.mod_small with (b:=two_p (Z.of_nat 64)).
+    rewrite Z.add_comm. rewrite Z_mod_plus_full.
+    rewrite Z.div_add.
+    rewrite Z.div_small. rewrite Z.add_0_l.
+    rewrite Z.mod_small.
+    rewrite decode_encode_reloctype. simpl.
+    rewrite Heqo. auto.
+    destruct rt;simpl;lia.
+    destruct rt;simpl;lia.
+    apply andb_true_iff in Heqb0. destruct Heqb0.
+    apply Z.ltb_lt in H10. apply Z.ltb_lt in H. lia.
+    simpl.
+    apply andb_true_iff in Heqb0. destruct Heqb0.
+    apply Z.ltb_lt in H10. apply Z.ltb_lt in H.
+    split.    
+    destruct rt;simpl;lia.
+    rewrite two_power_pos_equiv.
+    destruct rt;simpl;lia.
+  - destr_in H.
+    inv H. unfold encode_int32.
+    rewrite decode_encode_int.
+    
+    rewrite Z.mod_small with (b:=two_p (Z.of_nat 4*8)).
+    rewrite Z.add_comm. rewrite Z_mod_plus_full.
+    rewrite Z.div_add.
+    rewrite Z.div_small. rewrite Z.add_0_l.
+    rewrite Z.mod_small.
+    rewrite decode_encode_reloctype. simpl.
+    rewrite Heqo. auto.
+    destruct rt;simpl;lia.
+    destruct rt;simpl;lia.
+    apply andb_true_iff in Heqb0. destruct Heqb0.
+    apply Z.ltb_lt in H10. apply Z.ltb_lt in H. lia.
+    simpl.
+    apply andb_true_iff in Heqb0. destruct Heqb0.
+    apply Z.ltb_lt in H10. apply Z.ltb_lt in H.
+    split.    
+    destruct rt;simpl;lia.
+    rewrite two_power_pos_equiv.
+    destruct rt;simpl;lia.
+
+Qed.
+
+Definition decode_relocentry (m: ZTree.t ident) (l: list byte) : res relocentry :=
+  if Archi.ptr64 then
+    do (ofsbytes, l) <- take_drop 8 l;
+    do (infobytes, l) <- take_drop 8 l;
+    let ofs := decode_int ofsbytes in
+    do (rt, sym) <- decode_reloc_info m infobytes;
+    OK ({| reloc_offset := ofs; reloc_type := rt; reloc_symb := sym; reloc_addend := 0 |})
+  else
+    do (ofsbytes, l) <- take_drop 4 l;
+    do (infobytes, l) <- take_drop 4 l;
+    let ofs := decode_int ofsbytes in
+    do (rt, sym) <- decode_reloc_info m infobytes;
+    OK ({| reloc_offset := ofs; reloc_type := rt; reloc_symb := sym; reloc_addend := 0 |}).
