Makefile
@@ -135,7 +135,7 @@ BACKEND=\
 ENCODE=Encode.v Bits.v Hex.v BPProperty.v
 
 # Elf file format (unused: MergeSection.v)
-ELF = RelocElf.v EncodeRelocElf.v SymbtableEncode.v RelocElfgen.v ReloctablesEncode.v RemoveAddend.v RelocElfDecode.v
+ELF = RelocElf.v EncodeRelocElf.v SymbtableEncode.v RelocElfgen.v ReloctablesEncode.v RemoveAddend.v RelocElfSemantics.v ReloctablesDecode.v SymbtableDecode.v
 
 # CAV generation file
 AUTOGEN = VerificationCondition.v EncDecRet.v
